Otway-Rees: proved secrecy of conversation key for all states of honest principals
Also adapted the attacker functions "according to the changed protocol
definition".

otway-rees-fixed/OYRS.SecurityProps.fst
@@ -49,6 +49,7 @@ let responder_and_server_and_conv_key_stored_in_initiator_state
     | Success (APP ser_st) -> (
       match OYRS.Sessions.parse_session_st ser_st with
      | Success (InitiatorRecvedMsg4 srv b k_ab) -> (
+       srv = server /\
        b = responder /\
        k_ab = conv_key
      )
@@ -75,6 +76,7 @@ let initiator_and_server_and_conv_key_stored_in_responder_state
     | Success (APP ser_st) -> (
       match OYRS.Sessions.parse_session_st ser_st with
      | Success (ResponderSentMsg4 srv a k_ab) -> (
+       srv = server /\
        a = initiator /\
        k_ab = conv_key
      )
@@ -114,7 +116,20 @@ let conv_key_stored_in_initiator_state_is_secret
   responder
   server
   conv_key
-= secrecy_lemma #(pki oyrs_preds) conv_key
+=
+  match LabeledPKI.parse_session_st init_state.[state_session_idx] with
+  | Success (APP ser_st) -> (
+    match OYRS.Sessions.parse_session_st ser_st with
+    | Success (InitiatorRecvedMsg4 srv b k_ab) -> (
+      let now = global_timestamp () in
+      assert(later_than now set_state_idx);
+      assert(OYRS.Sessions.valid_session now initiator state_session_idx vv.[state_session_idx] (InitiatorRecvedMsg4 srv b k_ab));
+      assert((corrupt_id now (P initiator) \/ corrupt_id now (P server) \/ corrupt_id now (P responder) \/ is_labeled now k_ab (readers [P server; P initiator; P responder])));
+      secrecy_lemma #(pki oyrs_preds) conv_key
+    )
+    | _ -> ()
+  )
+  | _ -> ()
 
 let conv_key_stored_in_responder_state_is_secret
   responder
@@ -125,5 +140,15 @@ let conv_key_stored_in_responder_state_is_secret
   initiator
   server
   conv_key
-= secrecy_lemma #(pki oyrs_preds) conv_key
-
+=
+  match LabeledPKI.parse_session_st resp_state.[state_session_idx] with
+  | Success (APP ser_st) -> (
+    match OYRS.Sessions.parse_session_st ser_st with
+    | Success (ResponderSentMsg4 srv a k_ab) -> (
+      let now = global_timestamp () in
+      assert(later_than now set_state_idx);
+      secrecy_lemma #(pki oyrs_preds) conv_key
+    )
+    | _ -> ()
+  )
+  | _ -> ()
